moved tactics into CompileStmtTactics.v

platform/cito/VerifCondOk.v
@@ -19,16 +19,73 @@ Section TopSection.
   Variable modName : string.
 
   Require Import Syntax.
-
-  Variable s k : Stmt.
-
   Require Import Wrap.
 
+  Definition compile := compile layout vars temp_size imports_global modName.
+
   Lemma verifCond_ok : 
-    forall pre : assert,
+    forall (s k : Stmt) (pre : assert),
       vcs (verifCond layout vars temp_size s k pre) ->
       vcs
-        (VerifCond (compile layout vars temp_size imports_global modName s k pre)).
+        (VerifCond (compile s k pre)).
+  Proof.
+
+    Require Import Semantics.
+    Require Import Safe.
+    Require Import Notations.
+    Require Import SemanticsFacts.
+    Require Import ScopeFacts.
+    Require Import ListFacts.
+    Require Import StringSet.
+    Require Import SetFacts.
+    Require Import CompileStmtTactics.
+
+    Open Scope stmt.
+
+    Opaque funcs_ok.
+    Opaque mult.
+    Opaque star. (* necessary to use eapply_cancel *)
+
+    Hint Resolve Subset_in_scope_In.
+    Hint Extern 0 (Subset _ _) => progress (simpl; subset_solver).
+
+    unfold verifCond, imply; induction s.
+
+    (* skip *)
+    wrap0.
+
+    (* seq *)
+    wrap0.
+    eapply IHs1.
+    wrap0.
+    eapply H2 in H.
+    unfold precond in *.
+    unfold inv in *.
+    unfold inv_template in *.
+    post.
+    descend.
+    eauto.
+    eauto.
+    eapply Safe_Seq_assoc; eauto.
+    eauto.
+    eauto.
+    clear_imports.
+    repeat hiding ltac:(step auto_ext).
+    descend.
+    eapply RunsTo_Seq_assoc; eauto.
+    eapply in_scope_Seq_Seq; eauto.
+
+    eapply IHs2.
+    wrap0.
+    Require Import PostOk.
+    unfold compile in H.
+    unfold TopSection.compile in H.
+    eapply post_ok in H.
+    unfold postcond in *.
+    unfold inv in *.
+    unfold inv_template in *.
+    post.
+
     admit.
   Qed.
 
